Fix stale

Iris/Iris/Instances/Lib/LaterCredits.lean
@@ -1,9 +1,11 @@
 /-
 Copyright (c) 2026 Sergei Stepanenko. All rights reserved.
 Released under Apache 2.0 license as described in the file LICENSE.
+Authors: Sergei Stepanenko, Zongyuan Liu
 -/
 module
 
+public import Iris.Std.TC
 public import Iris.Algebra
 public import Iris.Algebra.Auth
 public import Iris.Algebra.Numbers
@@ -16,11 +18,16 @@ public import Iris.Instances.IProp
 namespace Iris
 
 open _root_.Std (Associative Commutative LeftIdentity LawfulLeftIdentity)
-open Iris OFE COFE BI Auth CommMonoidLike
+open Iris OFE COFE BI Auth CommMonoidLike Std
 
 section LcGS
 
 abbrev Credit := Nat
+
+@[rocq_alias has_lc]
+inductive HasLC? where
+| HasNoLC
+| HasLC
 
 scoped instance : Associative (Add.add (α := Credit)) := ⟨Nat.add_assoc⟩
 scoped instance : Commutative (Add.add (α := Credit)) := ⟨Nat.add_comm⟩
@@ -41,35 +48,63 @@ class LcGpreS (GF : BundledGFunctors) where
 
 attribute [reducible, instance] LcGpreS.lc_elem
 
-class LcGS (GF : BundledGFunctors) extends LcGpreS GF where
+class LcGS (hlc : outParam HasLC?) (GF : BundledGFunctors)  extends LcGpreS GF where
   lc_name : GName
 
 end LcGS
 
 section Definitions
 
-variable {GF : BundledGFunctors} [LC : LcGS GF]
+variable {GF : BundledGFunctors} {hlc : HasLC?} [LC : LcGS hlc GF]
 
+/-- The user-facing credit resource, denoting ownership of `i` credits
+(but only if later credits are enabled). -/
 def lc (i : Credit) : IProp GF :=
-  iOwn (E := LC.lc_elem) LC.lc_name (◯ i)
+  match hlc with
+  | .HasLC => iOwn (E := LC.lc_elem) LC.lc_name (◯ i)
+  | .HasNoLC => iprop(True)
 
 notation:max "£ " i:40 => lc i
 
+/-- The internal authoritative part of the credit ghost state, tracking how many
+credits are available in total. Users should not directly interface with this. -/
 def lc_supply (i : Credit) : IProp GF :=
-  iOwn (E := LC.lc_elem) LC.lc_name (● i)
+  match hlc with
+  | .HasLC => iOwn (E := LC.lc_elem) LC.lc_name (● i)
+  | .HasNoLC => iprop(⌜i = 0⌝)
 
 end Definitions
 
 section Operations
 
-variable {GF : BundledGFunctors} [LC : LcGS GF]
+variable {GF : BundledGFunctors} {hlc : HasLC?} [LC : LcGS hlc GF]
 
-theorem lc_split {n m} : £ (n + m) ⊣⊢@{IProp GF} £ n ∗ £ m :=
-  -- FIXME: Timeout on iOwn_op. Why?
-  iOwn_op (E := LC.lc_elem) (a1 := ◯ n) (a2 := ◯ m)
+theorem lc_split {n m} : £ (n + m) ⊣⊢@{IProp GF} £ n ∗ £ m := by
+  cases hlc with
+  | HasNoLC =>
+    simp only [lc]
+    exact (true_sep (P := iprop(True))).symm
+  | HasLC =>
+    -- FIXME: Timeout on iOwn_op. Why?
+    simp only [lc]
+    refine .trans ?_ iOwn_op
+    exact .rfl
+
+@[rocq_alias lc_no_lc]
+theorem lc_no_lc [LcGS .HasNoLC GF] (n : Credit) : £ n ⊣⊢@{IProp GF} iprop(True) := .rfl
+
+@[rocq_alias lc_supply_no_lc]
+theorem lc_supply_no_lc [LcGS .HasNoLC GF] (n : Credit) :
+    lc_supply n ⊣⊢@{IProp GF} iprop(⌜n = 0⌝) := .rfl
 
 @[rocq_alias lc_zero]
-theorem lc_zero : ⊢@{IProp GF} |==> £ 0 := iOwn_unit (ε := UCMRA.unit)
+theorem lc_zero : ⊢@{IProp GF} |==> £ 0 := by
+  cases hlc with
+  | HasNoLC => simp only [lc]; imodintro; ipure_intro; trivial
+  | HasLC => exact iOwn_unit (ε := UCMRA.unit)
+
+section LcSupplyRules
+variable [LC : LcGS .HasLC GF]
 
 @[rocq_alias lc_supply_bound]
 theorem lc_supply_bound {n m} : ⊢@{IProp GF} lc_supply m -∗ £ n -∗ ⌜n ≤ m⌝ := by
@@ -106,6 +141,8 @@ imod iOwn_update $$ H with Hown
 icases iOwn_op $$ Hown with ⟨Hm, _⟩
 iframe
 
+end LcSupplyRules
+
 @[rocq_alias lc_succ]
 theorem lc_succ {n} : £ (.succ n) ⊣⊢@{IProp GF} £ 1 ∗ £ n := by
   rw [show .succ n = 1 + n by simp [Nat.succ_eq_add_one, Nat.add_comm]]
@@ -121,12 +158,14 @@ theorem lc_weaken {n} m (h : m ≤ n) : ⊢@{IProp GF} £ n -∗ £ m := by
 @[rocq_alias lc_timeless]
 instance {n} : Timeless (PROP := IProp GF) (£ n) := by
   unfold lc
-  infer_instance
+  cases hlc <;> infer_instance
 
 @[rocq_alias lc_0_persistent]
 instance : Persistent (PROP := IProp GF) (£ 0) := by
   unfold lc
-  apply instPersistentIPropIOwnOfCoreIdAp
+  cases hlc
+  · infer_instance
+  · apply instPersistentIPropIOwnOfCoreIdAp
 
 end Operations
 
@@ -134,7 +173,7 @@ section ProofMode
 
 open ProofMode
 
-variable {GF : BundledGFunctors} [LcGS GF]
+variable {GF : BundledGFunctors} {hlc : HasLC?} [LcGS hlc GF]
 
 @[rocq_alias from_sep_lc_add]
 instance (priority := default - 10) {n m} : FromSep (PROP := IProp GF) (£ (n + m)) (£ n) (£ m) where
@@ -162,11 +201,14 @@ end ProofMode
 
 section Upd
 
-variable {GF : BundledGFunctors} [LcGS GF]
+variable {GF : BundledGFunctors} {hlc : HasLC?} [LcGS hlc GF]
 
 @[rocq_alias le_upd.le_upd_pre]
 def le_upd_pre (P le_upd : IProp GF) : IProp GF :=
-  iprop(∀ n, lc_supply n ==∗ (lc_supply n ∗ P) ∨ (∃ m, ⌜m < n⌝ ∗ lc_supply m ∗ ▷ le_upd))
+  iprop(∀ n, lc_supply n ==∗
+    ▷^[n.succ] False ∨
+    (lc_supply n ∗ P) ∨
+    (∃ m, ⌜m < n⌝ ∗ lc_supply m ∗ ▷ le_upd))
 
 @[rocq_alias le_upd.le_upd_pre_contractive]
 instance {P : IProp GF} : Contractive (le_upd_pre P) where
@@ -175,6 +217,7 @@ instance {P : IProp GF} : Contractive (le_upd_pre P) where
     refine forall_ne (fun i => ?_)
     refine wand_ne.ne .rfl ?_
     refine UPred.bupd_ne.ne ?_
+    refine or_ne.ne .rfl ?_
     refine or_ne.ne .rfl ?_
     refine exists_ne (fun m => ?_)
     refine sep_ne.ne .rfl ?_
@@ -198,7 +241,8 @@ delab_rule le_upd
 @[rocq_alias le_upd.le_upd_unfold]
 theorem le_upd_unfold {P : IProp GF} :
   (|==£> P) ⊣⊢
-  ∀ n, lc_supply n ==∗ (lc_supply n ∗ P) ∨ (∃ m, ⌜m < n⌝ ∗ lc_supply m ∗ ▷ |==£> P) :=
+  ∀ n, lc_supply n ==∗
+    ▷^[n.succ] False ∨ (lc_supply n ∗ P) ∨ (∃ m, ⌜m < n⌝ ∗ lc_supply m ∗ ▷ |==£> P) :=
     (equiv_iff.mp (fixpoint_unfold ⟨le_upd_pre P, inferInstance⟩)).trans .rfl
 
 @[rocq_alias le_upd.le_upd_ne]
@@ -211,6 +255,7 @@ instance : NonExpansive (le_upd (GF := GF)) where
     refine forall_ne (fun i => ?_)
     refine wand_ne.ne .rfl ?_
     refine UPred.bupd_ne.ne ?_
+    refine or_ne.ne .rfl ?_
     refine or_ne.ne (sep_ne.ne .rfl H) ?_
     refine exists_ne (fun m => ?_)
     refine sep_ne.ne .rfl ?_
@@ -218,13 +263,42 @@ instance : NonExpansive (le_upd (GF := GF)) where
     refine Contractive.distLater_dist ?_
     exact (fun k Hk => IH k Hk (H.lt Hk))
 
+@[rocq_alias le_upd.le_upd_unfold_no_le]
+theorem le_upd_unfold_no_le [LcGS .HasNoLC GF] {P : IProp GF} : (|==£> P) ⊣⊢ |==> ◇ P := by
+  apply le_upd_unfold.trans
+  constructor
+  · iintro H
+    ihave Hs : lc_supply 0 $$ []
+    · iapply (lc_supply_no_lc 0).mpr; ipure_intro; rfl
+    imod H $$ %0 Hs with (HFalse | ⟨_, HP⟩ | ⟨%m, %Hlt, _⟩)
+    · imodintro
+      icases (laterN_later 0).mp $$ HFalse with HFalse
+      icases laterN_0.mp $$ HFalse with HFalse
+      simp only [BIBase.except0]
+      ileft
+      iexact HFalse
+    · imodintro; iapply except0_intro $$ HP
+    · exact absurd Hlt m.not_lt_zero
+  · iintro H %n Hn
+    icases (lc_supply_no_lc n).mp $$ Hn with %Hn
+    subst Hn
+    imod H
+    simp only [BIBase.except0]
+    icases H with (HFalse | HP)
+    · imodintro; ileft
+      iapply (laterN_later 0).mpr
+      inext; iexact HFalse
+    · imodintro; iright; ileft
+      iframe HP
+      iapply (lc_supply_no_lc 0).mpr; ipure_intro; rfl
+
 @[rocq_alias le_upd.bupd_le_upd]
 theorem bupd_le_upd {P : IProp GF} : (|==> P) ⊢ (|==£> P) := by
   iintro H
   iapply le_upd_unfold
   iintro %n Hsupp
   imod H; imodintro
-  ileft
+  iright; ileft
   isplitl [Hsupp] <;> iassumption
 
 @[rocq_alias le_upd.le_upd_intro]
@@ -240,30 +314,31 @@ theorem le_upd_bind {P Q : IProp GF} : ⊢ (P -∗ |==£> Q) -∗ (|==£> P) -�
   iintro HLöb H G
   iapply le_upd_unfold
   iintro %n Hsupp
-  imod le_upd_unfold $$ G Hsupp with (⟨Hsupp, G⟩|⟨%m, %Hlt, Hsupp, G⟩)
+  imod le_upd_unfold $$ G Hsupp with (HFalse|⟨Hsupp, G⟩|⟨%m, %Hlt, Hsupp, G⟩)
+  · imodintro; ileft; iexact HFalse
   · ihave G := H $$ G
-    imod le_upd_unfold $$ G Hsupp with (⟨Hsupp, G⟩|⟨%m, %Hlt, Hsupp, G⟩)
+    imod le_upd_unfold $$ G Hsupp with (HFalse|⟨Hsupp, G⟩|⟨%m, %Hlt, Hsupp, G⟩)
+    · imodintro; ileft; iexact HFalse
     · imodintro
-      ileft
-      isplitl [Hsupp] <;> iassumption
+      iright; ileft
+      iframe
     · imodintro
-      iright
+      iright; iright
       iexists m
-      isplit
-      · ipure_intro; assumption
-      isplitl [Hsupp] <;> iassumption
+      iframe
+      ipure_intro; assumption
   · imodintro
-    iright
+    iright; iright
     iexists m
+    iframe
     isplit
     · ipure_intro; assumption
-    isplitl [Hsupp]; iassumption
     inext
     iapply HLöb $$ H G
   ipure_intro; simp
 
-@[rocq_alias le_upd.le_upd_later_elim]
-theorem le_upd_later_elim {P : IProp GF} : ⊢ £ 1 -∗ (▷ |==£> P) -∗ |==£> P := by
+@[rocq_alias le_upd.lc_le_upd_elim_later]
+theorem le_upd_later_elim [LcGS .HasLC GF] {P : IProp GF} : ⊢ £ 1 -∗ (▷ |==£> P) -∗ |==£> P := by
   iintro Hcr H
   iapply le_upd_unfold
   iintro %n Hsupp
@@ -274,11 +349,10 @@ theorem le_upd_later_elim {P : IProp GF} : ⊢ £ 1 -∗ (▷ |==£> P) -∗ |==
     rw [show n.succ = 1 + n by omega]
     imod lc_decrease_supply $$ Hsupp Hcr with Hsupp
     imodintro
-    iright
+    iright; iright
     iexists n
-    isplit
-    · ipure_intro; simp
-    isplitr [H] <;> iassumption
+    iframe
+    ipure_intro; simp
 
 @[rocq_alias le_upd.le_upd_mono]
 theorem le_upd_mono {P Q : IProp GF} (Hent : P ⊢ Q) : (|==£> P) ⊢ (|==£> Q) := by
@@ -292,7 +366,7 @@ theorem le_upd_mono {P Q : IProp GF} (Hent : P ⊢ Q) : (|==£> P) ⊢ (|==£> Q
 theorem le_upd_trans {P : IProp GF} : (|==£> |==£> P) ⊢ |==£> P := by
   iintro H
   iapply le_upd_bind $$ [] H
-  iintro H; iexact H
+  iintro $
 
 @[rocq_alias le_upd.le_upd_frame_r]
 theorem le_upd_frame_r {P R : IProp GF} : (|==£> P) ∗ R ⊢ |==£> (P ∗ R) := by
@@ -300,7 +374,7 @@ theorem le_upd_frame_r {P R : IProp GF} : (|==£> P) ∗ R ⊢ |==£> (P ∗ R) 
   iapply le_upd_bind $$ [HR] H
   iintro HP
   iapply le_upd_intro
-  isplitl [HP] <;> iassumption
+  iframe
 
 @[rocq_alias le_upd.le_upd_frame_l]
 theorem le_upd_frame_l {P R : IProp GF} : R ∗ (|==£> P) ⊢ |==£> (R ∗ P) := by
@@ -308,24 +382,24 @@ theorem le_upd_frame_l {P R : IProp GF} : R ∗ (|==£> P) ⊢ |==£> (R ∗ P) 
   refine (.trans sep_comm.mp ?_)
   iapply le_upd_frame_r
 
-@[rocq_alias le_upd.le_upd_later]
-theorem le_upd_later {P : IProp GF} : ⊢ £ 1 -∗ ▷ P -∗ |==£> P := by
+@[rocq_alias le_upd.lc_le_upd_add_later]
+theorem le_upd_later [LcGS .HasLC GF] {P : IProp GF} : ⊢ £ 1 -∗ ▷ P -∗ |==£> P := by
   iintro H1 H2
   iapply le_upd_later_elim $$ H1
   inext
   iapply le_upd_intro $$ H2
 
 @[rocq_alias le_upd.except_0_le_upd]
-theorem except_0_le_upd {P : IProp GF} : ◇ (|==£> P) ⊢ |==£> (◇ P) := by
+theorem except_0_le_upd {P : IProp GF} : ◇ (|==£> P) ⊢ |==£> P := by
   simp only [BIBase.except0]
-  iintro (H|H)
-  · iapply le_upd_intro
-    ileft
-    iexact H
-  · iapply le_upd_mono $$ H
-    iintro H
-    iright
-    iexact H
+  iintro (HFalse | $)
+  iapply le_upd_unfold
+  iintro %n _
+  imodintro
+  ileft
+  iapply (laterN_later n).mpr
+  inext
+  iexact HFalse
 
 end Upd
 
@@ -333,73 +407,17 @@ section Internal
 
 open ProofMode
 
-variable {GF : BundledGFunctors} [LcGS GF]
+variable {GF : BundledGFunctors} {hlc : HasLC?} [LcGS hlc GF]
 
-@[rocq_alias le_upd.le_upd_elim]
-theorem le_upd_elim n (P : IProp GF) :
-  ⊢@{IProp GF} lc_supply n -∗ (|==£> P) -∗
-    n.repeat (fun P => iprop(|==> ▷ P)) iprop(|==> ◇ (∃ m, ⌜m ≤ n⌝ ∗ lc_supply m ∗ P)) := by
-  apply WellFounded.induction Nat.lt_wfRel.wf n
-  intro n IH
-  iintro Ha Hupd
-  icases le_upd_unfold $$ Hupd with Hupd
-  ihave Hupd := Hupd $$ %n Ha
-  cases n with
-  | zero =>
-    simp only [Nat.le_zero_eq, Nat.repeat]
-    imod Hupd with (⟨Ha, HP⟩|⟨%m, %Hlt, _⟩)
-    · imodintro; imodintro
-      iexists 0
-      isplit
-      · ipure_intro; rfl
-      isplitl [Ha] <;> iassumption
-    · exfalso; exact m.not_lt_zero Hlt
-  | succ n =>
-    simp only [Nat.repeat]
-    imod Hupd with (⟨Hc, HP⟩|Hupd)
-    · imodintro; inext
-      iapply iter_modal_intro $$ [Hc HP]
-      · intro Q; iintro H; imodintro; inext; iexact H
-      imodintro; imodintro
-      iexists n.succ
-      isplit
-      · ipure_intro; exact Nat.le_refl _
-      isplitl [Hc] <;> iassumption
-    · imodintro
-      icases Hupd with ⟨%m, ⟨%Hstep, ⟨Hown, LaterHupd⟩⟩⟩
-      obtain ⟨k, Heq⟩ := Nat.exists_eq_add_of_lt Hstep
-      rw [show n = m + k by exact Nat.add_right_cancel Heq, Nat.repeat_add]
-      inext
-      ihave IH := IH m (by simp [WellFoundedRelation.rel]; omega) $$ Hown LaterHupd
-      iapply iter_modal_mono $$ [] IH
-      · iintro %P %Q H HP; imod HP; imodintro; inext; iapply H $$ HP
-      iintro IH
-      iapply iter_modal_intro $$ [IH]
-      · iintro %Q H; imodintro; inext; iexact H
-      imod IH; imodintro
-      imod IH with ⟨%m', %Hlt, H1, H2⟩; imodintro
-      iexists m'
-      isplit
-      · ipure_intro
-        grind
-      isplitl [H1] <;> iassumption
+omit [LcGS hlc GF] in
+/-- `▷^[1] False` (i.e. `▷ False`) entails `◇ X`: it is the left disjunct of the except-0 modality. -/
+private theorem except0_intro_false {X : IProp GF} : iprop(▷^[1] False) ⊢ iprop(◇ X) :=
+  or_intro_l
 
-@[rocq_alias le_upd.le_upd_elim_complete]
-theorem le_upd_elim_complete n (P : IProp GF) :
-    ⊢ lc_supply n -∗ (|==£> P) -∗ n.succ.repeat (fun Q => iprop(|==> ▷ Q)) P := by
-  iintro Hlc Hupd
-  ihave Hit := le_upd_elim n P $$ Hlc Hupd
-  rw [show Nat.succ n = n + 1 by omega, Nat.repeat_add]
-  iapply iter_modal_mono $$ [] Hit
-  · iintro %P %Q Hent HP
-    imod HP; imodintro; inext
-    iapply Hent $$ HP
-  simp only [Nat.repeat]
-  iintro Hupd
-  imod Hupd; imodintro
-  imod Hupd; inext
-  icases Hupd with ⟨%m, ⟨_, ⟨_, HP⟩⟩⟩
-  iexact HP
+omit [LcGS hlc GF] in
+private theorem laterN_succ_false_except0 {X : IProp GF} (n : Nat) :
+    iprop(▷^[n.succ] False) ⊢ iprop(▷^[n] ◇ X) :=
+  (laterN_later n).mp.trans (laterN_mono n or_intro_l)
 
 @[rocq_alias le_upd.elim_bupd_le_upd]
 instance {P : IProp GF} : ElimModal True p false (bupd P) P (le_upd Q) (le_upd Q) where
@@ -429,12 +447,8 @@ instance {P : IProp GF} [H : FromPure a P io φ] : FromPure a (le_upd P) io φ w
       iapply H.from_pure $$ H
 
 @[rocq_alias le_upd.is_except_0_le_upd]
-instance {P : IProp GF} [H : IsExcept0 P] : IsExcept0 (le_upd P) where
-  is_except0 := by
-    iintro G
-    icases except_0_le_upd $$ G with G
-    iapply le_upd_mono $$ G
-    iapply H.is_except0
+instance {P : IProp GF} : IsExcept0 (le_upd P) where
+  is_except0 := except_0_le_upd
 
 @[rocq_alias le_upd.from_modal_le_upd]
 instance {P : IProp GF} : FromModal True modality_id (le_upd P) (le_upd P) P where
@@ -459,23 +473,33 @@ instance {p} {P R Q : IProp GF} [hf : Frame p R P Q] : Frame p R (le_upd P) (le_
 end Internal
 
 @[rocq_alias le_upd.lc_alloc]
-theorem lc_alloc [H : LcGpreS GF] n : ⊢@{IProp GF} |==> ∃ _ : LcGS GF, lc_supply n ∗ £ n := by
+theorem lc_alloc [H : LcGpreS GF] n : ⊢@{IProp GF} |==> ∃ _ : LcGS .HasLC GF, lc_supply n ∗ £ n := by
   imod (iOwn_alloc (E := H.lc_elem) ((● n) • (◯ n)) (auth_both_valid.mpr ⟨fun _ => .rfl, ⟨⟩⟩))
     with ⟨%γLC, HOwn⟩
   icases iOwn_op $$ HOwn with ⟨HAuth, HFrag⟩
-  let LC : LcGS GF := { lc_elem := H.lc_elem, lc_name := γLC }
+  let LC : LcGS .HasLC GF := { lc_elem := H.lc_elem, lc_name := γLC }
   iexists LC
   imodintro
   simp only [lc_supply, lc]
   isplitl [HAuth] <;> iassumption
 
-@[rocq_alias le_upd_finally]
-def le_upd_finally [LcGS GF] (P : IProp GF) : IProp GF :=
+@[rocq_alias le_upd.lc_alloc_no_lc]
+theorem lc_alloc_no_lc [H : LcGpreS GF] n :
+    ⊢@{IProp GF} ∃ _ : LcGS .HasNoLC GF, lc_supply 0 ∗ £ n := by
+  let LC : LcGS .HasNoLC GF := { lc_elem := H.lc_elem, lc_name := default }
+  iexists LC
+  simp only [lc_supply, lc]
+  isplitr []
+  · ipure_intro; trivial
+  ipure_intro; trivial
+
+@[rocq_alias le_upd.le_upd_finally]
+def le_upd_finally [LcGS hlc GF] (P : IProp GF) : IProp GF :=
   iprop(∀ m, lc_supply m -∗ ▷^[m] ◇ ■ P)
 
-#rocq_ignore le_upd_finally_aux "Not needed"
-#rocq_ignore le_upd_finally_def "Not needed"
-#rocq_ignore le_upd_finally_unseal "Not needed"
+#rocq_ignore le_upd.le_upd_finally_aux "Not needed"
+#rocq_ignore le_upd.le_upd_finally_def "Not needed"
+#rocq_ignore le_upd.le_upd_finally_unseal "Not needed"
 
 syntax:max "|==£|> " term:40 : term
 
@@ -486,9 +510,9 @@ delab_rule le_upd_finally
 | `($_ $P) => do ``(iprop(|==£|> $(← unpackIprop P)))
 
 section le_upd_finally_rules
-variable [LcGS GF]
+variable {hlc : HasLC?} [LcGS hlc GF]
 
-@[rocq_alias le_upd_finally_ne]
+@[rocq_alias le_upd.le_upd_finally_ne]
 instance le_upd_finally_ne : NonExpansive (le_upd_finally (GF := GF)) where
   ne _ _ _ H := by
     simp only [le_upd_finally]
@@ -498,7 +522,7 @@ instance le_upd_finally_ne : NonExpansive (le_upd_finally (GF := GF)) where
     refine except0_ne.ne ?_
     exact instPlainly_ne.ne H
 
-@[rocq_alias le_upd_finally_mono]
+@[rocq_alias le_upd.le_upd_finally_mono]
 theorem le_upd_finally_mono (P Q: IProp GF) : (P ⊢ Q) → (|==£|> P) ⊢ (|==£|> Q) := by
   intro Hent
   unfold le_upd_finally
@@ -510,21 +534,21 @@ theorem le_upd_finally_mono (P Q: IProp GF) : (P ⊢ Q) → (|==£|> P) ⊢ (|==
   iintro HP
   iapply plainly_mono Hent $$ HP
 
-@[rocq_alias le_upd_finally_intro]
+@[rocq_alias le_upd.le_upd_finally_intro]
 theorem le_upd_finally_intro (P : IProp GF) : ■ P ⊢ |==£|> P := by
   unfold le_upd_finally
   iintro HP %m _Hlc
   iapply laterN_intro
-  iapply except0_intro
-  iexact HP
+  iapply except0_intro $$ HP
 
-@[rocq_alias le_upd_finally_finally]
+@[rocq_alias le_upd.le_upd_le_upd_finally]
 theorem le_upd_le_upd_finally (P : IProp GF) : (|==£> |==£|> P) ⊢ |==£|> P := by
-  iapply BILoeb.loeb_weak
   unfold le_upd_finally
-  iintro IH HP %m Hlc
+  iintro HP %m Hlc
+  iloeb as IH generalizing %m
   icases le_upd_unfold $$ HP with HP
-  imod HP $$ Hlc with ⟨⟨Hlc, H⟩ | ⟨%m', %Hm, Hlc , H⟩⟩
+  imod HP $$ Hlc with ⟨HFalse | ⟨Hlc, H⟩ | ⟨%m', %Hm, Hlc , H⟩⟩
+  · iapply laterN_succ_false_except0 $$ HFalse
   · iapply H; iframe
   conv =>
     rhs
@@ -532,19 +556,8 @@ theorem le_upd_le_upd_finally (P : IProp GF) : (|==£> |==£|> P) ⊢ |==£|> P 
   iapply laterN_add; inext
   iapply laterN_add; inext
   iapply IH $$ H Hlc
-  ipure_intro;trivial
 
-@[rocq_alias except_0_le_upd_finally]
-theorem except0_le_upd_finally (P : IProp GF) : (◇ |==£|> P) ⊢ |==£|> P := by
-  unfold le_upd_finally
-  iintro HP %m Hlc
-  iapply laterN_mono _ (except0_idemp (P := iprop(■ P))).mp
-  iapply except0_laterN
-  imod HP
-  imodintro
-  iapply HP;iassumption
-
-@[rocq_alias le_upd_finally_except_0]
+@[rocq_alias le_upd.le_upd_finally_except_0]
 theorem le_upd_finally_except0 (P : IProp GF) : (|==£|> ◇ P) ⊢ |==£|> P := by
   unfold le_upd_finally
   iintro HP %m Hlc
@@ -552,7 +565,7 @@ theorem le_upd_finally_except0 (P : IProp GF) : (|==£|> ◇ P) ⊢ |==£|> P :=
   iapply laterN_mono _ (except0_mono except0_plainly.mpr)
   iapply HP $$ Hlc
 
-@[rocq_alias le_upd_finally_add_lc]
+@[rocq_alias le_upd.le_upd_finally_add_lc]
 theorem le_upd_finally_add_lc (P : IProp GF) : (£ 1 -∗ |==£|> P) ⊢ |==£|> ▷ ◇ P := by
   unfold le_upd_finally
   iintro H %m Hlc
@@ -560,207 +573,118 @@ theorem le_upd_finally_add_lc (P : IProp GF) : (£ 1 -∗ |==£|> P) ⊢ |==£|>
   iapply laterN_mono _ later_plainly.mp
   iapply laterN_mono _ (later_mono except0_plainly.mp)
   iapply (laterN_later m).mp
-  rw [show m + 1 = 1 + m from Nat.add_comm m 1]
-  imod lc_increase_supply 1 $$ Hlc with ⟨Hlc, Hl⟩
-  iapply H $$ Hl Hlc
-
--- TODO: move
-omit [LcGS GF] in
-private theorem timeless_laterN {X : IProp GF} [Timeless X] (n : Nat) :
-    iprop(▷^[n] X) ⊢ iprop(▷^[n] False ∨ X) := by
-  induction n with
-  | zero => exact or_intro_r
-  | succ n IH =>
-    -- ▷^[n+1] X = ▷ ▷^[n] X ⊢ ▷ (▷^[n] False ∨ X)
-    refine (later_mono IH).trans ?_
-    -- ▷ (▷^[n] False ∨ X) ⊣⊢ ▷ ▷^[n] False ∨ ▷ X = ▷^[n+1] False ∨ ▷ X
-    refine later_or.mp.trans ?_
-    -- Timeless: ▷ X ⊢ ▷ False ∨ X
-    refine or_mono .rfl Timeless.timeless |>.trans ?_
-    -- ▷ False ⊢ ▷^[n+1] False (via later_mono (laterN_intro n))
-    refine or_mono .rfl (or_mono_l (later_mono (laterN_intro n))) |>.trans ?_
-    -- ▷^[n+1] False ∨ ▷^[n+1] False ∨ X ⊢ ▷^[n+1] False ∨ X
-    exact or_assoc.mpr.trans (or_mono or_self.mp .rfl)
-
-@[rocq_alias le_upd_finally_keep]
-theorem le_upd_finally_keep (P Q : IProp GF) [Timeless P] : (|==£|> P) ∧ (P -∗ |==£|> Q) ⊢ |==£|> Q := by
-  unfold le_upd_finally
-  iintro H %m Hlc
-  ihave #HP : ▷^[m] ◇ ■ P $$ [H Hlc]
-  · icases H with ⟨H, -⟩
-    iapply H $$ Hlc
-  icases H with ⟨-, H⟩
-  icases (laterN_mono _ except0_into_later) $$ HP with HP
-  icases (laterN_later _).mpr $$ HP with HP
-  icases (timeless_laterN _) $$ HP with HP
-  icases HP with (HFalse | HP')
-  · icases (laterN_later _).mp $$ HFalse with HFalse
+  cases hlc with
+  | HasLC =>
+    rw [show m + 1 = 1 + m from Nat.add_comm m 1]
+    imod lc_increase_supply 1 $$ Hlc with ⟨Hlc, Hl⟩
+    iapply H $$ Hl Hlc
+  | HasNoLC =>
+    icases (lc_supply_no_lc m) $$ Hlc with %Hlc
+    subst Hlc
+    rw [Nat.zero_add]
     inext
-    imod HFalse
-    iexfalso; iassumption
-  iapply H $$ HP' Hlc
+    ihave Hone : £ 1 $$ []
+    · iapply (lc_no_lc 1).mpr; ipure_intro; trivial
+    ihave Hz : lc_supply 0 $$ []
+    · iapply (lc_supply_no_lc 0).mpr; ipure_intro; rfl
+    ispecialize H $$ Hone %0 Hz
+    iapply laterN_0
+    iassumption
 
-@[rocq_alias le_upd_finally_forall]
+@[rocq_alias le_upd.le_upd_finally_forall]
 theorem le_upd_finally_forall (Φ : A → IProp GF) : (∀ x, |==£|> Φ x) ⊢ |==£|> ∀ x, Φ x := by
   unfold le_upd_finally
   iintro H %m Hlc %x
   iapply H $$ Hlc
 
-    -- (** Derived rules *)
-    -- (** Since the modality is used only internally in the version for fancy
-    -- updates, we do not provide instances of the proof mode classes. *)
-
-    -- Global Instance le_upd_finally_proper : Proper ((⊣⊢) ==> (⊣⊢)) le_upd_finally.
-    -- Proof. apply: ne_proper. Qed.
-    -- Global Instance le_upd_finally_mono' : Proper ((⊢) ==> (⊢)) le_upd_finally.
-    -- Proof. intros P Q. apply le_upd_finally_mono. Qed.
-    -- Global Instance le_upd_finally_flip_mono' :
-    --   Proper (flip (⊢) ==> flip (⊢)) le_upd_finally.
-    -- Proof. intros P Q. apply le_upd_finally_mono. Qed.
-
-@[rocq_alias le_upd_finally_later]
-theorem le_upd_finally_later (P : IProp GF) : ▷ (|==£|> P) ⊢ |==£|> ▷ ◇ P := by
+@[rocq_alias le_upd.le_upd_keep]
+theorem le_upd_keep (P Q : IProp GF) [TCOr (TCEq hlc .HasNoLC) (Timeless P)] :
+    (|==£|> P) ∧ (P -∗ |==£> Q) ⊢ |==£> Q := by
   iintro H
-  iapply le_upd_finally_add_lc
-  iintro Hl
-  iapply le_upd_le_upd_finally
-  iapply le_upd_later $$ Hl H
+  iapply le_upd_unfold
+  iintro %n Hc
+  ihave #⟨$| HP⟩ : iprop((▷^[n.succ] False) ∨ ■ P) $$ [H Hc]
+  · icases H with ⟨H, -⟩
+    unfold le_upd_finally
+    cases ‹TCOr (TCEq hlc .HasNoLC) (Timeless P)› with
+    | r =>
+      iapply timeless_laterN
+      ispecialize H $$ Hc
+      icases (laterN_mono n except0_into_later) $$ H with H
+      icases (laterN_later _).mpr $$ H with $
+    | l =>
+      cases ‹TCEq hlc .HasNoLC›
+      icases (lc_supply_no_lc n).mp $$ Hc with %Hn
+      subst n
+      ispecialize H $$ Hc
+      icases laterN_0.mp $$ H with H
+      rw [← Nat.add_one]
+      rw [eq_of_eqv <| equiv_iff.mpr <| laterN_later (n := 0)]
+      rw [eq_of_eqv <| equiv_iff.mpr <| laterN_0]
+      unfold BIBase.except0
+      iapply H
+  icases H with ⟨-, H⟩
+  ispecialize H $$ HP
+  iapply le_upd_unfold $$ H
+  iframe
+
+#rocq_ignore le_upd_finally_proper "Subsumed by the NonExpansive instance `le_upd_finally_ne`"
+#rocq_ignore le_upd_finally_mono' "Subsumed by `le_upd_finally_mono`"
+#rocq_ignore le_upd_finally_flip_mono' "Subsumed by `le_upd_finally_mono`"
+
+@[rocq_alias le_upd.le_upd_finally_later]
+theorem le_upd_finally_later (P : IProp GF) : ▷ (|==£|> P) ⊢ |==£|> ▷ ◇ P := by
+  unfold le_upd_finally
+  iintro H %m Hlc
+  -- `▷ ◇ ■ P ⊢ ◇ ■ (▷ ◇ P)`: `■ (▷ ◇ P) ⊣⊢ ▷ ◇ ■ P`, then introduce the `◇`.
+  have hbody : iprop(▷ ◇ ■ P) ⊢ iprop(◇ ■ (▷ ◇ P)) :=
+    except0_intro.trans <| except0_mono <|
+      (later_mono except0_plainly.1).trans <| later_plainly.1
+  -- Goal `▷^[m] ◇ ■ (▷ ◇ P)` ⟸ `▷^[m] (▷ ◇ ■ P) = ▷^[m+1] ◇ ■ P = ▷ (▷^[m] ◇ ■ P)`.
+  iapply laterN_mono _ hbody
+  iapply (laterN_later m).mp
+  iapply (later_laterN m).mpr
+  inext
+  iapply H $$ Hlc
 
 end le_upd_finally_rules
 
-theorem le_upd_finally_soundness [LcGpreS GF] n (P : IProp GF) :
-  (∀ [LcGS GF], £ n ⊢ |==£|> P) → ⊢ P := by
+@[rocq_alias le_upd.le_upd_finally_soundness]
+theorem le_upd_finally_soundness (hlc : HasLC?) [LcGpreS GF] n (P : IProp GF) :
+  (∀ [LcGS hlc GF], £ n ⊢ |==£|> P) → ⊢ P := by
   intro HP
-  apply laterN_soundness (n := n.succ)
-  iintro _
-  iapply (laterN_later _).mpr
-  iapply (laterN_mono _ except0_into_later)
-  iapply (laterN_mono _ (except0_mono plainly_elim))
-  imod lc_alloc n with ⟨%LC, Hlc, Hl⟩
-  have HP' : £ n ⊢ iprop(∀ m, lc_supply m -∗ ▷^[m] ◇ ■ P) := HP
-  iapply HP' $$ Hl Hlc
+  cases hlc with
+  | HasLC =>
+    apply laterN_soundness (n := n.succ)
+    iintro _
+    iapply (laterN_later _).mpr
+    iapply (laterN_mono _ except0_into_later)
+    iapply (laterN_mono _ (except0_mono plainly_elim))
+    imod lc_alloc n with ⟨%LC, Hlc, Hl⟩
+    have HP' : £ n ⊢ iprop(∀ m, lc_supply m -∗ ▷^[m] ◇ ■ P) := HP
+    iapply HP' $$ Hl Hlc
+  | HasNoLC =>
+    apply laterN_soundness (n := 1)
+    iintro _
+    iapply (laterN_later 0).mpr
+    iapply laterN_0.mpr
+    iapply later_mono plainly_elim
+    iapply except0_into_later
+    icases lc_alloc_no_lc n with ⟨%LC, Hlc, Hl⟩
+    unfold le_upd_finally at HP
+    ihave G := HP $$ Hl %0 Hlc
+    iapply laterN_0.mp $$ G
 
 @[rocq_alias le_upd.lc_soundness]
-theorem lc_soundness [LcGpreS GF] m (P : IProp GF) [Plain P]  (H : ∀ {_: LcGS GF}, ⊢ £ m -∗ |==£> P) :
-    ⊢ P := by
-  apply laterN_soundness (n := m.succ)
-  refine .trans ?_ bupd_elim
-  iintro emp; iclear emp
-  imod lc_alloc m with ⟨%γ, H1, H2⟩
-  -- FIXME: Is it possible to support nested specializations? le_upd_elim_complete $$ H1 (H $$ H2)?
-  ihave G := H $$ H2
-  ihave G := le_upd_elim_complete $$ H1 G
-  simp only [Nat.succ_eq_add_one, Nat.repeat]
-  imod G; imodintro
-  -- TODO: inext is too eager to remove all laters from the goal
-  iapply later_laterN; inext
-  clear H
-  istop
-  induction m with
-  | zero => simpa only [Nat.zero_eq, Nat.repeat] using .rfl
-  | succ m IH =>
-    simp only [Nat.succ_eq_add_one, Nat.repeat]
-    iintro H
-    iapply later_laterN
-    iapply bupd_elim
-    imod H; imodintro; inext
-    exact IH
-
-section If
-
-open ProofMode
-
-variable {GF : BundledGFunctors} [LcGS GF]
-
-@[rocq_alias le_upd_if.le_upd_if]
-def le_upd_if (b : Bool) : IProp GF → IProp GF :=
-  if b then le_upd else bupd
-
-@[rocq_alias le_upd_if.le_upd_if_ne]
-instance le_upd_if_ne : NonExpansive (le_upd_if b (GF := GF)) := by
-  cases b <;> (simp only [le_upd_if, Bool.false_eq_true, ↓reduceIte]; infer_instance)
-
-@[rocq_alias le_upd_if.le_upd_if_mono']
-theorem le_upd_if_mono {P Q : IProp GF} : (P ⊢ Q) → (le_upd_if b P) ⊢ (le_upd_if b Q) := by
-  cases b <;> (simp only [le_upd_if, Bool.false_eq_true, ↓reduceIte])
-  · intro H; iintro G
-    imod G; imodintro; iapply H $$ G
-  · apply le_upd_mono
-
-@[rocq_alias le_upd_if.le_upd_if_intro]
-theorem le_upd_if_intro {b} {P : IProp GF} : P ⊢ le_upd_if b P := by
-  cases b <;> (simp only [le_upd_if, Bool.false_eq_true, ↓reduceIte])
-  · iintro H; imodintro; iassumption
-  · apply le_upd_intro
-
-@[rocq_alias le_upd_if.le_upd_if_bind]
-theorem le_upd_if_bind {b} {P Q : IProp GF} :
-    ⊢ (P -∗ le_upd_if b Q) -∗ (le_upd_if b P) -∗ (le_upd_if b Q) := by
-  cases b <;> (simp only [le_upd_if, Bool.false_eq_true, ↓reduceIte])
-  · iintro H G
-    imod G
-    iapply H $$ G
-  · apply le_upd_bind
-
-@[rocq_alias le_upd_if.le_upd_if_trans]
-theorem le_upd_if_trans {b} {P : IProp GF} : (le_upd_if b (le_upd_if b P)) ⊢ le_upd_if b P := by
-  cases b <;> (simp only [le_upd_if, Bool.false_eq_true, ↓reduceIte])
-  · apply bupd_idem.mp
-  · apply le_upd_trans
-
-@[rocq_alias le_upd_if.le_upd_if_frame_r]
-theorem le_upd_if_frame_r {b} {P R : IProp GF} : (le_upd_if b P) ∗ R ⊢ le_upd_if b iprop(P ∗ R) := by
-  cases b <;> (simp only [le_upd_if, Bool.false_eq_true, ↓reduceIte])
-  · apply bupd_frame_r
-  · apply le_upd_frame_r
-
-@[rocq_alias le_upd_if.bupd_le_upd_if]
-theorem bupd_le_upd_if {b} {P : IProp GF} : (|==> P) ⊢ (le_upd_if b P) := by
-  cases b <;> (simp only [le_upd_if, Bool.false_eq_true, ↓reduceIte])
-  · exact .rfl
-  · apply bupd_le_upd
-
-@[rocq_alias le_upd_if.le_upd_if_frame_l]
-theorem le_upd_if_frame_l {b} {R Q : IProp GF} : (R ∗ le_upd_if b Q) ⊢ le_upd_if b iprop(R ∗ Q) := by
-  cases b <;> (simp only [le_upd_if, Bool.false_eq_true, ↓reduceIte])
-  · apply bupd_frame_l
-  · apply le_upd_frame_l
-
-@[rocq_alias le_upd_if.except_0_le_upd_if]
-theorem except_0_le_upd_if {b} {P : IProp GF} : ◇ (le_upd_if b P) ⊢ le_upd_if b iprop(◇ P) := by
-  cases b <;> (simp only [le_upd_if, Bool.false_eq_true, ↓reduceIte])
-  · apply bupd_except0
-  · apply except_0_le_upd
-
-@[rocq_alias le_upd_if.elim_bupd_le_upd_if]
-instance {b} {p} {P Q : IProp GF} : ElimModal True p false (bupd P) P (le_upd_if b Q) (le_upd_if b Q) := by
-  cases b <;> (simp only [le_upd_if, Bool.false_eq_true, ↓reduceIte]; infer_instance)
-
-@[rocq_alias le_upd_if.from_pure_le_upd_if]
-instance {b} {a} {P : IProp GF} φ [FromPure a P io φ] : FromPure a (le_upd_if b P) io φ := by
-  cases b <;> (simp only [le_upd_if, Bool.false_eq_true, ↓reduceIte]; infer_instance)
-
-@[rocq_alias le_upd_if.is_except_0_le_upd_if]
-instance {b} {P : IProp GF} [IsExcept0 P] : IsExcept0 (le_upd_if b P) := by
-  cases b <;> (simp only [le_upd_if, Bool.false_eq_true, ↓reduceIte]; infer_instance)
-
-@[rocq_alias le_upd_if.from_modal_le_upd_if]
-instance {b} {P : IProp GF} : FromModal True modality_id (le_upd_if b P) (le_upd_if b P) P := by
-  cases b <;> (simp only [le_upd_if, Bool.false_eq_true, ↓reduceIte]; infer_instance)
-
-@[rocq_alias le_upd_if.elim_modal_le_upd_if]
-instance {b} {p} {P Q : IProp GF} :
-  ElimModal True p false (le_upd_if b P) P (le_upd_if b Q) (le_upd_if b Q) := by
-  cases b <;> (simp only [le_upd_if, Bool.false_eq_true, ↓reduceIte]; infer_instance)
-
-@[rocq_alias le_upd_if.frame_le_upd_if]
-instance {p b} {P R Q : IProp GF} [hf : Frame p R P Q] : Frame p R (le_upd_if b P) (le_upd_if b Q) where
-  frame := le_upd_if_frame_l.trans <| le_upd_if_mono hf.frame
-
-@[rocq_alias le_upd_if.from_assumption_le_upd_if]
-instance from_assumption_le_upd_if {p} {P Q : IProp GF} [h : FromAssumption p ioP P Q] : FromAssumption p ioP P (le_upd_if b Q) where
-  from_assumption := h.1.trans le_upd_if_intro
-
-end If
+theorem lc_soundness (hlc : HasLC?) [LcGpreS GF] m (P : IProp GF) [Plain P]
+    (H : ∀ {_ : LcGS hlc GF}, ⊢ £ m -∗ |==£> P) : ⊢ P := by
+  apply le_upd_finally_soundness hlc m
+  intro LC
+  iintro Hcr
+  iapply le_upd_le_upd_finally
+  imod H $$ Hcr with HP
+  imodintro
+  iapply le_upd_finally_intro
+  iapply plain_plainly_2 $$ HP
 
 end Iris
